PropositionalLogic/Sound_Kripke.v
@@ -9,6 +9,7 @@ Require Import Logic.PropositionalLogic.KripkeSemantics.
 Require Import Logic.PropositionalLogic.IntuitionisticPropositionalLogic.
 Require Import Logic.PropositionalLogic.ClassicalPropositionalLogic.
 Require Import Logic.PropositionalLogic.GodelDummettLogic.
+Require Import Logic.PropositionalLogic.WeakClassicalLogic.
 
 Local Open Scope logic_base.
 Local Open Scope syntax.
@@ -189,6 +190,32 @@ Proof.
     tauto.
 Qed.
 
+Lemma sound_weak_excluded_middle_branch_join {L: Language} {nL: NormalLanguage L} {pL: PropositionalLanguage L} {MD: Model} {kMD: KripkeModel MD} {M: Kmodel} {kiM: KripkeIntuitionisticModel (Kworlds M)} {bkiM: BranchJoinKripkeIntuitionisticModel (Kworlds M)} {SM: Semantics L MD} {kiSM: KripkeIntuitionisticSemantics L MD M SM}:
+  forall x: expr,
+    forall m, KRIPKE: M, m |= ~~ x || ~~ ~~ x.
+Proof.
+  intros.
+  unfold negp.
+  rewrite sat_orp, !sat_impp.
+  apply Classical_Prop.NNPP; intro.
+  apply not_or_and in H; destruct H.
+  apply not_all_ex_not in H.
+  apply not_all_ex_not in H0.
+  destruct H as [n1 ?], H0 as [n2 ?].
+  apply imply_to_and in H.
+  apply imply_to_and in H0.
+  destruct H, H0.
+  apply imply_to_and in H1.
+  apply imply_to_and in H2.
+  destruct H1 as [? _], H2 as [? _].
+  destruct (Korder_branch_join n1 n2 m H H0) as [n [? ?]].
+  eapply sat_mono in H2; [| eassumption].
+  eapply sat_mono in H1; [| eassumption].
+  rewrite sat_impp in H2.
+  apply (H2 n) in H1; [| reflexivity].
+  apply sat_falsep in H1; auto.
+Qed.
+
 Theorem sound_intuitionistic_kripke_all (Var: Type): sound (IntuitionisticPropositionalLogic.G Var) (KripkeSemantics.SM Var) (AllModel _).
 Proof.
   hnf; intros.
@@ -249,7 +276,7 @@ Proof.
   + apply sound_excluded_middle_ident.
 Qed.
 
-Theorem sound_weak_classical_kripke_no_branch (Var: Type): sound 
+Theorem sound_godel_dummett_kripke_no_branch (Var: Type): sound 
 (GodelDummettPropositionalLogic.G Var) (KripkeSemantics.SM Var)
 (@KripkeModelClass (KripkeSemantics.MD Var) (KripkeSemantics.kMD Var) (KripkeSemantics.Kmodel_NoBranch Var)).
 Proof.
@@ -279,4 +306,36 @@ Proof.
   + apply sound_orp_elim.
   + apply sound_falsep_elim.
   + apply sound_impp_choice_no_branch.
+Qed.
+
+Theorem sound_weak_classical_kripke_branch_join (Var: Type): sound 
+(WeakClassicalLogic.G Var) (KripkeSemantics.SM Var)
+(@KripkeModelClass (KripkeSemantics.MD Var) (KripkeSemantics.kMD Var) (KripkeSemantics.Kmodel_BranchJoin Var)).
+Proof.
+  hnf; intros.
+  pose (PropositionalLanguage.L Var) as L.
+  pose (PropositionalLanguage.nL Var: NormalLanguage L) as nL.
+  pose (PropositionalLanguage.pL Var: PropositionalLanguage L) as pL.
+  pose (KripkeSemantics.MD Var) as MD.
+  pose (KripkeSemantics.kMD Var: KripkeModel MD) as kMD.
+  intros m ?.
+  destruct H0.
+  unfold KripkeSemantics.Kmodel_BranchJoin in H0.
+  rename H0 into bkiM.
+  pose (KripkeSemantics.kiM Var M: KripkeIntuitionisticModel (Kworlds M)) as kiM.
+  pose (KripkeSemantics.SM Var: Semantics L MD) as SM.
+  pose (KripkeSemantics.kiSM Var M: KripkeIntuitionisticSemantics L MD M SM) as kiSM.
+  induction H.
+  + pose proof sound_modus_ponens x y m.
+    exact (H1 IHprovable1 IHprovable2).
+  + apply sound_axiom1.
+  + apply sound_axiom2.
+  + apply sound_andp_intros.
+  + apply sound_andp_elim1. 
+  + apply sound_andp_elim2.
+  + apply sound_orp_intros1.
+  + apply sound_orp_intros2.
+  + apply sound_orp_elim.
+  + apply sound_falsep_elim.
+  + apply sound_weak_excluded_middle_branch_join.
 Qed.
